Extracted IntegerIntervals to separate module and generalized them

ulib/FStar.Algebra.CommMonoid.Fold.fst
@@ -1,5 +1,5 @@
 (*
-   Copyright 2008-2018 Microsoft Research
+   Copyright 2008-2022 Microsoft Research
    
    Licensed under the Apache License, Version 2.0 (the "License");
    you may not use this file except in compliance with the License.
@@ -17,10 +17,13 @@
 *)
 
 module FStar.Algebra.CommMonoid.Fold
+module CE = FStar.Algebra.CommMonoid.Equiv
 
 open FStar.Seq.Base
-open FStar.Seq.Properties
+open FStar.Seq.Properties 
 open FStar.Seq.Permutation
+
+open FStar.IntegerIntervals
 
 (* Here we define the notion for big sums and big products for 
    arbitrary commutative monoids. We construct the folds from 
@@ -28,98 +31,82 @@ open FStar.Seq.Permutation
    a sum or a product, depending on the monoid operation. *)
  
 (* We refine multiplication a bit to make proofs smoothier *)
-let ( *) (x y: int) : (t:int{(x>0 /\ y>0) ==> t>0}) = op_Multiply x y
- 
-type under (k: pos) = x:nat{x<k}
-type not_less_than (x: int) = (t: int{t>=x})
-type inbetween (x: int) (y: not_less_than x) = (t: int{t>=x && t<=y})
-type counter_of_range (x: int) (y: not_less_than x) = (t: nat{t<(y+1-x)})
 
-let range_count (x: int) (y: not_less_than x) : pos = (y+1)-x
- 
-(* This lemma, especially when used with forall_intro, helps the 
-   prover verify the index ranges of sequences that correspond 
-   to arbitrary big_sums *)
-let bounds_lemma (n0:int) (nk: not_less_than n0) (i: counter_of_range n0 nk) 
-  : Lemma (n0+i >= n0 /\ n0+i <= nk) = ()
-  
+open FStar.Mul  
+
+(* Notice how we can't just use a and b if we don't want to break 
+   recursive calls with the same exprs *)
 let init_func_from_expr #c (#n0: int) (#nk: not_less_than n0) 
-                        (expr: (inbetween n0 nk) -> c) 
-                        (a: inbetween n0 nk) 
-                        (b: inbetween a nk) 
-  : ((counter_of_range a b) -> c)
-  = fun (i: counter_of_range a b) -> expr (n0+i)
+                        (expr: (ifrom_ito n0 nk) -> c) 
+                        (a: ifrom_ito n0 nk) (b: ifrom_ito a nk) 
+  : (counter_for (ifrom_ito a b) -> c)
+  = fun (i: counter_for (ifrom_ito a b)) -> expr (n0 + i)
   
-type comm_monoid c eq = Algebra.CommMonoid.Equiv.cm c eq 
-
 (* 
-   Fold (Big Σ or Big Π notation in mathematics) of an arbitrary 
+   Fold (Big Sum or Big Product notation in mathematics) of an arbitrary 
    function expr defined over a finite range of integers.
 
    Notice how one should very strictly control the domains of 
    lambdas, otherwise the proofs easily fail. 
 *)
 let rec fold #c #eq 
-             (cm: comm_monoid c eq) 
-             (n0: int) 
-             (nk: not_less_than n0) 
-             (expr: (inbetween n0 nk) -> c) 
-  : Pure c (requires True)  
-           (ensures (fun (x:c) -> ((nk = n0) ==> (x == expr nk)))) 
-           (decreases nk-n0) = 
-  if nk = n0 then expr nk
-  else (fold cm n0 (nk-1) expr) `cm.mult` expr nk
+             (cm: CE.cm c eq) 
+             (a: int) (b: not_less_than a) 
+             (expr: (ifrom_ito a b) -> c) 
+  // some of the lemmas want (ensures (fun (x:c) -> ((nk = n0) ==> (x == expr nk)))) 
+  : Tot (c) (decreases b-a) 
+  = if b = a then expr b
+    else (fold cm a (b-1) expr) `cm.mult` expr b
 
 (* This lemma establishes the definitional equality of the fold 
    given said equality for all the values from the allowed range *)
-let rec fold_equality #c #eq (cm: comm_monoid c eq) 
-  (n0: int) (nk: int{nk>=n0}) (expr1 expr2: (inbetween n0 nk)->c)
-  : Lemma (requires (forall (i: inbetween n0 nk). expr1 i == expr2 i))
-          (ensures fold cm n0 nk expr1 == fold cm n0 nk expr2)
-          (decreases nk-n0) = 
-  if nk>n0 then fold_equality cm n0 (nk-1) expr1 expr2 
+let rec fold_equality #c #eq (cm: CE.cm c eq) 
+  (a: int) (b: not_less_than a) 
+  (expr1 expr2: (ifrom_ito a b) -> c)
+  : Lemma (requires (forall (i: ifrom_ito a b). expr1 i == expr2 i))
+          (ensures fold cm a b expr1 == fold cm a b expr2)
+          (decreases b - a) = 
+  if b > a then fold_equality cm a (b - 1) expr1 expr2 
   
 (* This lemma decomposes the big_sum into the sum of the first 
    (k-1) elements plus the remaining last one.
    Obviously requires the argument range that is at least 
    2 elements long. *)
 let fold_snoc_decomposition #c #eq 
-  (cm: comm_monoid c eq) 
-  (n0: int) 
-  (nk: int{nk > n0}) 
-  (expr: (inbetween n0 nk) -> c) 
-  : Lemma (fold cm n0 nk expr == 
-           fold cm n0 (nk-1) expr `cm.mult` (expr nk)) = ()
+  (cm: CE.cm c eq) 
+  (a: int) (b: greater_than a) 
+  (expr: (ifrom_ito a b) -> c) 
+  : Lemma (fold cm a b expr == fold cm a (b-1) expr `cm.mult` (expr b)) = ()
 
 (* This lemma establishes the equality of fold over int range to its
    seq-based foldm_snoc counterpart. *)
 let rec fold_equals_seq_foldm #c #eq  
-                             (cm: comm_monoid c eq) 
-                             (n0: int) 
-                             (nk: not_less_than n0) 
-                             (expr: (inbetween n0 nk) -> c)
-  : Lemma (ensures fold cm n0 nk expr `eq.eq` 
-                   foldm_snoc cm (init (range_count n0 nk) 
-                                       (init_func_from_expr expr n0 nk)))
-          (decreases nk-n0) = 
-  if (nk=n0) then (
-   let ts = init (range_count n0 nk) (init_func_from_expr expr n0 nk) in
-   lemma_eq_elim (create 1 (expr nk)) ts; 
-   Seq.Permutation.foldm_snoc_singleton cm (expr nk);   
-   eq.symmetry (foldm_snoc cm ts) (expr nk);
-   eq.reflexivity (expr nk); 
-   eq.transitivity (fold cm n0 nk expr) (expr nk) (foldm_snoc cm ts)
+                             (cm: CE.cm c eq) 
+                             (a: int) 
+                             (b: not_less_than a) 
+                             (expr: (ifrom_ito a b) -> c)
+  : Lemma (ensures fold cm a b expr `eq.eq` 
+                   foldm_snoc cm (init (closed_interval_size a b) 
+                                       (init_func_from_expr expr a b)))
+          (decreases b-a) = 
+  if (b=a) then (
+   let ts = init (closed_interval_size a b) (init_func_from_expr expr a b) in
+   lemma_eq_elim (create 1 (expr b)) ts; 
+   foldm_snoc_singleton cm (expr b);   
+   eq.symmetry (foldm_snoc cm ts) (expr b);
+   eq.reflexivity (expr b); 
+   eq.transitivity (fold cm a b expr) (expr b) (foldm_snoc cm ts)
   )
   else (
-    let lhs = fold cm n0 nk expr in
-    let fullseq = init (range_count n0 nk) (init_func_from_expr expr n0 nk) in    
+    let lhs = fold cm a b expr in
+    let fullseq = init (closed_interval_size a b) (init_func_from_expr expr a b) in    
     let rhs = foldm_snoc cm fullseq in
-    let subseq = init (range_count n0 (nk-1)) (init_func_from_expr expr n0 (nk-1)) in
-    let subsum = fold cm n0 (nk-1) expr in 
+    let subseq = init (closed_interval_size a (b-1)) (init_func_from_expr expr a (b-1)) in
+    let subsum = fold cm a (b-1) expr in 
     let subfold = foldm_snoc cm subseq in
-    let last = expr nk in
+    let last = expr b in
     let op = cm.mult in
-    fold_equals_seq_foldm cm n0 (nk-1) expr;    
+    fold_equals_seq_foldm cm a (b-1) expr;    
     lemma_eq_elim (fst (un_snoc fullseq)) subseq;
     cm.commutativity last subfold;
     eq.reflexivity last; 
